# Matrix Multiplication

Given two matrices $A$ (shape $m \times n$) and $B$ (shape $n \times p$), the product $C = AB$ results in a matrix of shape $m \times p$. Each element $C_{ij}$ is the dot product of the $i$-th row of $A$ and the $j$-th column of $B$:

$$ C_{ij} = \sum_{k} A_{ik} B_{kj} $$

**Walkthrough of the example below:**

$$
\begin{bmatrix} 1 & 2 \\ 3 & 4 \end{bmatrix} \cdot \begin{bmatrix} 5 & 6 \\ 7 & 8 \end{bmatrix} = \begin{bmatrix} (1 \cdot 5 + 2 \cdot 7) & (1 \cdot 6 + 2 \cdot 8) \\ (3 \cdot 5 + 4 \cdot 7) & (3 \cdot 6 + 4 \cdot 8) \end{bmatrix}
$$

*   Row 1, Col 1: $1 \times 5 + 2 \times 7 = 5 + 14 = 19$
*   Row 1, Col 2: $1 \times 6 + 2 \times 8 = 6 + 16 = 22$
*   Row 2, Col 1: $3 \times 5 + 4 \times 7 = 15 + 28 = 43$
*   Row 2, Col 2: $3 \times 6 + 4 \times 8 = 18 + 32 = 50$

# Inverse of a Matrix

**Mathematical Definition:**

The inverse of a square matrix $A$ is a matrix $A^{-1}$ such that their product is the identity matrix $I$ (a matrix with 1s on the diagonal and 0s elsewhere):

$$ A \cdot A^{-1} = A^{-1} \cdot A = I $$

For a $2 \times 2$ matrix $A = \begin{bmatrix} a & b \\ c & d \end{bmatrix}$, the inverse exists if the determinant $\det(A) = ad - bc \neq 0$. The formula is:

$$ A^{-1} = \frac{1}{\det(A)} \begin{bmatrix} d & -b \\ -c & a \end{bmatrix} = \frac{1}{ad-bc} \begin{bmatrix} d & -b \\ -c & a \end{bmatrix} $$

**Walkthrough of the example below:**

Given $A = \begin{bmatrix} 1 & 2 \\ 3 & 4 \end{bmatrix}$:

1.  **Calculate Determinant:** $\det(A) = (1)(4) - (2)(3) = 4 - 6 = -2$.
2.  **Apply Formula:**
    $$ A^{-1} = \frac{1}{-2} \begin{bmatrix} 4 & -2 \\ -3 & 1 \end{bmatrix} = \begin{bmatrix} -2 & 1 \\ 1.5 & -0.5 \end{bmatrix} $$

# Pseudo-Inverse of a Matrix

**Mathematical Definition:**

The Moore-Penrose pseudo-inverse $A^+$ exists for any matrix $A$ (not necessarily square or invertible). It is a generalization of the inverse. If $A$ is invertible, $A^+ = A^{-1}$.

The pseudo-inverse provides a way to solve systems like $Ax = b$ that may not have a unique solution or any solution at all (in the least-squares sense).

Common formula (when columns are linearly independent, i.e., $A^T A$ is invertible):

$$ A^+ = (A^T A)^{-1} A^T $$